CellularAutomatas/proofs/two_stage_is_rt_closed.lean
@@ -10,6 +10,54 @@ variable {α Γ : Type} [Alphabet α] [Alphabet Γ]
 open CellAutomaton
 
 
+
+def TwoStageAdvice.L {α} [Alphabet α] (adv: TwoStageAdvice α Bool): Language α :=
+  { w: Word α | (adv.advice w).getLast? = true }
+
+
+def TwoStageAdvice.to_CA_rt {α} [Alphabet α] (adv: TwoStageAdvice α Bool): CA_rt α :=
+  fix_empty false (toRtCa $ adv.C.map_project (fun q => adv.M.f (adv.M.δ adv.M.q0 q)))
+
+
+
+@[simp]
+lemma TwoStageAdvice.to_CA_rt_L {α} [Alphabet α] (adv: TwoStageAdvice α Bool):
+    adv.to_CA_rt.val.L = adv.L := by
+  ext w
+
+  unfold TwoStageAdvice.to_CA_rt
+  unfold TwoStageAdvice.L
+  rw [Set.mem_setOf_eq]
+
+  by_cases h_empty: w = []
+  · simp [h_empty]
+
+  simp [h_empty]
+  rw [←trace_rt_L h_empty]
+  unfold TwoStageAdvice.advice
+  simp
+
+  erw [←FiniteStateTransducer.getLast?_of_scanr]
+  grind
+
+
+
+
+def TwoStageAdvice.from_CA_rt {α} [Alphabet α] (C: CA_rt α): TwoStageAdvice α Bool :=
+  {
+    β := Bool
+    C := C.val.toCellAutomaton
+    M := FiniteStateTransducer.M_id Bool
+  }
+
+@[simp]
+lemma TwoStageAdvice.from_CA_rt_spec {α} [Alphabet α] (C: CA_rt α):
+    (TwoStageAdvice.from_CA_rt C).advice = C.val.trace_rt := by
+  funext w
+  simp [TwoStageAdvice.from_CA_rt, TwoStageAdvice.advice]
+
+
+
 theorem two_stage_is_rt_closed (adv: TwoStageAdvice α Γ):
     adv.advice.rt_closed := by
   rw [advice_rt_closed_iff]
@@ -34,13 +82,13 @@ theorem two_stage_is_rt_closed (adv: TwoStageAdvice α Γ):
     · unfold C'
       simp [h_empty]
 
-    · calc
-        w ∈ C'.val.L
-        _ ↔ w ∈ (fix_empty (decide ([] ∈ C.val.L)) combined.to_CA_rt).val.L := by simp [C']
-        _ ↔ w ∈ combined.L := by simp [h_empty]
-        _ ↔ List.getLast? (combined.advice w) = some true := by
-          unfold TwoStageAdvice.L
-          rw [Set.mem_setOf_eq]
-        _ ↔ w ⨂ adv.advice w ∈ C.val.L := by
-          rw [elemL_iff_trace_rt (by simp)]
-          simp [combined, h_empty]
+    calc
+      w ∈ C'.val.L
+      _ ↔ w ∈ (fix_empty (decide ([] ∈ C.val.L)) combined.to_CA_rt).val.L := by simp [C']
+      _ ↔ w ∈ combined.L := by simp [h_empty]
+      _ ↔ List.getLast? (combined.advice w) = some true := by
+        unfold TwoStageAdvice.L
+        rw [Set.mem_setOf_eq]
+      _ ↔ w ⨂ adv.advice w ∈ C.val.L := by
+        rw [elemL_iff_trace_rt (by simp)]
+        simp [combined, h_empty]
